A bunch of misc minor pushes forward

10ChainedEnvironment/Chaining.thy
@@ -2,11 +2,37 @@ theory Chaining
   imports ChainedEnvironment "../09HeapMemory/HeapMemory"
 begin
 
-definition unstack_list :: "(ptr \<times> ptr) heap \<Rightarrow> ptr \<Rightarrow> ptr list" where
-  "unstack_list env p = undefined"
+abbreviation chain_structured :: "(ptr \<times> ptr) heap \<Rightarrow> bool" where
+  "chain_structured h \<equiv> heap_all (\<lambda>p (v, p'). p' \<le> p) h"
+
+primrec chained_frame :: "(ptr \<times> ptr) heap \<Rightarrow> (ptr \<times> nat) \<Rightarrow> bool" where
+  "chained_frame env (p, pc) = hcontains env p"
+
+abbreviation chained_stack :: "(ptr \<times> ptr) heap \<Rightarrow> (ptr \<times> nat) list \<Rightarrow> bool" where
+  "chained_stack env sfs \<equiv> list_all (chained_frame env) sfs"
+
+primrec chained_closure :: "(ptr \<times> ptr) heap \<Rightarrow> ceclosure \<Rightarrow> bool" where
+  "chained_closure env (CEConst n) = True"
+| "chained_closure env (CELam p pc) = hcontains env p"
+
+abbreviation chained_closures :: "(ptr \<times> ptr) heap \<Rightarrow> ceclosure heap \<Rightarrow> bool" where
+  "chained_closures env h \<equiv> heap_all (\<lambda>p c. chained_closure env c) h"
+
+primrec chained_state :: "chained_state \<Rightarrow> bool" where
+  "chained_state (CES h env vs sfs cd) = (
+    chain_structured env \<and> chained_closures env h \<and> chained_stack env sfs)"
+
+fun unstack_list :: "(ptr \<times> ptr) heap \<Rightarrow> ptr \<Rightarrow> ptr list" where
+  "unstack_list env 0 = []"
+| "unstack_list env (Suc p) = (case hlookup env p of 
+      (v, p') \<Rightarrow> v # (if p' \<le> p then unstack_list env p' else undefined))"
+
+primrec unchain_closure :: "(ptr \<times> ptr) heap \<Rightarrow> ceclosure \<Rightarrow> hclosure" where
+  "unchain_closure env (CEConst k) = HConst k"
+| "unchain_closure env (CELam p pc) = HLam (unstack_list env p) pc"
 
 definition unchain_heap :: "ceclosure heap \<Rightarrow> (ptr \<times> ptr) heap \<Rightarrow> hclosure heap" where
-  "unchain_heap h env = undefined"
+  "unchain_heap h env = hmap (unchain_closure env) h"
 
 primrec unchain_frame :: "(ptr \<times> ptr) heap \<Rightarrow> (ptr \<times> nat) \<Rightarrow> (ptr list \<times> nat)" where
   "unchain_frame env (p, pc) = (unstack_list env p, pc)"
@@ -17,26 +43,77 @@ abbreviation unchain_stack :: "(ptr \<times> ptr) heap \<Rightarrow> (ptr \<time
 primrec unchain_state :: "chained_state \<Rightarrow> heap_state" where
   "unchain_state (CES h env vs sfs cd) = HS (unchain_heap h env) vs (unchain_stack env sfs) cd"
 
-lemma [simp]: "lookup (unstack_list env p) x = chain_lookup env p x"
-  by simp
+lemma [simp]: "unchain_heap hempty env = hempty"
+  by (simp add: unchain_heap_def)
+
+lemma [simp]: "chain_structured env \<Longrightarrow> hcontains env p \<Longrightarrow>
+  lookup (unstack_list env p) x = chain_lookup env p x"
+proof (induction env p x rule: chain_lookup.induct)
+  case (3 h p x)
+  thus ?case
+  proof (cases "hlookup h p")
+    case (Pair v p')
+    moreover from 3 have "hcontains h p" by auto
+    moreover from 3 have "chain_structured h" by simp
+    ultimately have X: "p' \<le> p" using heap_lookup_all by fastforce
+    with 3 have "hcontains h p'" by fastforce
+    with 3 Pair X show ?thesis by simp
+  qed
+qed (simp_all split: prod.splits)
 
 lemma [simp]: "halloc h (CEConst k) = (h', p) \<Longrightarrow> 
-    halloc (unchain_heap h env) (HConst k) = (unchain_heap h' env, p)"
-  by simp
+  halloc (unchain_heap h env) (HConst k) = (unchain_heap h' env, p)"
+proof -
+  assume "halloc h (CEConst k) = (h', p)"
+  hence "halloc (hmap (unchain_closure env) h) (unchain_closure env (CEConst k)) = 
+    (hmap (unchain_closure env) h', p)" by (metis halloc_map)
+  thus ?thesis by (simp add: unchain_heap_def)
+qed
 
 lemma [simp]: "halloc h (CELam p pc) = (h', v) \<Longrightarrow> 
-    halloc (unchain_heap h env) (HLam (unstack_list env p) pc) = (unchain_heap h' env, v)"
-  by simp
+  halloc (unchain_heap h env) (HLam (unstack_list env p) pc) = (unchain_heap h' env, v)"
+proof -
+  assume "halloc h (CELam p pc) = (h', v)"
+  hence "halloc (hmap (unchain_closure env) h) (unchain_closure env (CELam p pc)) = 
+    (hmap (unchain_closure env) h', v)" by (metis halloc_map)
+  thus ?thesis by (simp add: unchain_heap_def)
+qed
+
+lemma [simp]: "hlookup h x = CEConst k \<Longrightarrow> hcontains h x \<Longrightarrow> 
+    hlookup (unchain_heap h env) x = HConst k"
+  by (simp add: unchain_heap_def)
+
+lemma [simp]: "hlookup h x = CELam p pc \<Longrightarrow> hcontains h x \<Longrightarrow> 
+    hlookup (unchain_heap h env) x = HLam (unstack_list env p) pc"
+  by (simp add: unchain_heap_def)
+
+lemma unchain_state_reverse [simp]: "HS h vs sfs cd = unchain_state \<Sigma> \<Longrightarrow> 
+  \<exists>h\<^sub>c\<^sub>e env sfs\<^sub>c\<^sub>e. \<Sigma> = CES h\<^sub>c\<^sub>e env vs sfs\<^sub>c\<^sub>e cd \<and> h = unchain_heap h\<^sub>c\<^sub>e env \<and> 
+    sfs = unchain_stack env sfs\<^sub>c\<^sub>e"
+  by (induction \<Sigma>) simp_all
 
 theorem completece [simp]: "unchain_state \<Sigma>\<^sub>c\<^sub>e \<leadsto>\<^sub>h \<Sigma>\<^sub>h \<Longrightarrow> \<exists>\<Sigma>\<^sub>c\<^sub>e'. \<Sigma>\<^sub>c\<^sub>e \<leadsto>\<^sub>c\<^sub>e \<Sigma>\<^sub>c\<^sub>e' \<and> \<Sigma>\<^sub>h = unchain_state \<Sigma>\<^sub>c\<^sub>e'"
   by simp
 
-theorem correctce [simp]: "\<Sigma>\<^sub>c\<^sub>e \<leadsto>\<^sub>c\<^sub>e \<Sigma>\<^sub>c\<^sub>e' \<Longrightarrow> unchain_state \<Sigma>\<^sub>c\<^sub>e \<leadsto>\<^sub>h unchain_state \<Sigma>\<^sub>c\<^sub>e'"
+lemma [simp]: "iter (\<leadsto>\<^sub>h) (unchain_state \<Sigma>\<^sub>c\<^sub>e) \<Sigma>\<^sub>h \<Longrightarrow> 
+  \<exists>\<Sigma>\<^sub>c\<^sub>e'. iter (\<leadsto>\<^sub>c\<^sub>e) \<Sigma>\<^sub>c\<^sub>e \<Sigma>\<^sub>c\<^sub>e' \<and> \<Sigma>\<^sub>h = unchain_state \<Sigma>\<^sub>c\<^sub>e'"
+proof (induction "unchain_state \<Sigma>\<^sub>c\<^sub>e" \<Sigma>\<^sub>h arbitrary: \<Sigma>\<^sub>c\<^sub>e rule: iter.induct)
+  case (iter_step \<Sigma>\<^sub>h' \<Sigma>\<^sub>h'')
+  then obtain \<Sigma>\<^sub>c\<^sub>e' where "\<Sigma>\<^sub>c\<^sub>e \<leadsto>\<^sub>c\<^sub>e \<Sigma>\<^sub>c\<^sub>e' \<and> \<Sigma>\<^sub>h' = unchain_state \<Sigma>\<^sub>c\<^sub>e'" by fastforce
+  moreover with iter_step obtain \<Sigma>\<^sub>c\<^sub>e'' where "iter (\<leadsto>\<^sub>c\<^sub>e) \<Sigma>\<^sub>c\<^sub>e' \<Sigma>\<^sub>c\<^sub>e'' \<and> \<Sigma>\<^sub>h'' = unchain_state \<Sigma>\<^sub>c\<^sub>e''" 
+    by fastforce
+  ultimately have "iter (\<leadsto>\<^sub>c\<^sub>e) \<Sigma>\<^sub>c\<^sub>e \<Sigma>\<^sub>c\<^sub>e'' \<and> \<Sigma>\<^sub>h'' = unchain_state \<Sigma>\<^sub>c\<^sub>e''" by fastforce
+  then show ?case by fastforce
+qed force+
+
+theorem correctce [simp]: "\<Sigma>\<^sub>c\<^sub>e \<leadsto>\<^sub>c\<^sub>e \<Sigma>\<^sub>c\<^sub>e' \<Longrightarrow> chained_state \<Sigma>\<^sub>c\<^sub>e \<Longrightarrow> 
+  unchain_state \<Sigma>\<^sub>c\<^sub>e \<leadsto>\<^sub>h unchain_state \<Sigma>\<^sub>c\<^sub>e'"
 proof (induction \<Sigma>\<^sub>c\<^sub>e \<Sigma>\<^sub>c\<^sub>e' rule: evalce.induct)
   case (evce_apply cd pc h v2 p' pc' env v1 env' p'' vs p sfs)
   from evce_apply have "cd ! pc = BApply" by simp
   from evce_apply have "hlookup h v2 = CELam p' pc'" by simp
   from evce_apply have "halloc env (v1, p') = (env', p'')" by simp
+  from evce_apply have "chain_structured env \<and> hcontains env p \<and> chained_stack env sfs" by simp
 
   from evce_apply have "hlookup (unchain_heap h env) v2 = HLam (unstack_list env p') pc' \<Longrightarrow>
         HS (unchain_heap h env) (v1 # v2 # vs) ((unstack_list env p, Suc pc) # unchain_stack env sfs) cd \<leadsto>\<^sub>h
@@ -48,6 +125,31 @@ proof (induction \<Sigma>\<^sub>c\<^sub>e \<Sigma>\<^sub>c\<^sub>e' rule: evalce
 next
   case (evce_jump cd pc h v2 p' pc' env v1 env' p'' vs p sfs)
   then show ?case by simp
+qed simp_all
+
+lemma [simp]: "halloc env (v, p') = (env', p) \<Longrightarrow> p' \<le> p \<Longrightarrow> chain_structured env \<Longrightarrow> 
+    chain_structured env'"
+  by auto
+
+lemma [simp]: "halloc env (v, p') = (env', p) \<Longrightarrow> chained_frame env f \<Longrightarrow> chained_frame env' f"
+  by (induction f) simp_all
+
+lemma [simp]: "halloc env (v, p') = (env', p) \<Longrightarrow> chained_stack env sfs \<Longrightarrow> 
+    chained_stack env' sfs"
+  by (induction sfs) simp_all
+
+lemma [simp]: "\<Sigma>\<^sub>c\<^sub>e \<leadsto>\<^sub>c\<^sub>e \<Sigma>\<^sub>c\<^sub>e' \<Longrightarrow> chained_state \<Sigma>\<^sub>c\<^sub>e \<Longrightarrow> chained_state \<Sigma>\<^sub>c\<^sub>e'"
+  apply (induction \<Sigma>\<^sub>c\<^sub>e \<Sigma>\<^sub>c\<^sub>e' rule: evalce.induct)
+  apply auto
+  by simp
+
+lemma [simp]: "iter (\<leadsto>\<^sub>c\<^sub>e) \<Sigma>\<^sub>c\<^sub>e \<Sigma>\<^sub>c\<^sub>e' \<Longrightarrow> chained_state \<Sigma>\<^sub>c\<^sub>e \<Longrightarrow> 
+  iter (\<leadsto>\<^sub>h) (unchain_state \<Sigma>\<^sub>c\<^sub>e) (unchain_state \<Sigma>\<^sub>c\<^sub>e')"
+proof (induction \<Sigma>\<^sub>c\<^sub>e \<Sigma>\<^sub>c\<^sub>e' rule: iter.induct)
+  case (iter_step \<Sigma>\<^sub>c\<^sub>e \<Sigma>\<^sub>c\<^sub>e' \<Sigma>\<^sub>c\<^sub>e'')
+  hence "iter (\<leadsto>\<^sub>h) (unchain_state \<Sigma>\<^sub>c\<^sub>e') (unchain_state \<Sigma>\<^sub>c\<^sub>e'')" by simp
+  moreover from iter_step have "unchain_state \<Sigma>\<^sub>c\<^sub>e \<leadsto>\<^sub>h unchain_state \<Sigma>\<^sub>c\<^sub>e'" by simp
+  ultimately show ?case by simp
 qed simp_all
 
 end
