11FlatMemory/MemoryFlattening.thy
@@ -2,14 +2,69 @@ theory MemoryFlattening
   imports FlatMemory "../09HeapMemory/HeapConversion"
 begin
 
+primrec flatten_closure :: "ceclosure \<Rightarrow> nat list" where
+  "flatten_closure (CEConst k) = [0, k, 0]"
+| "flatten_closure (CELam p pc) = [1, 2 * p, pc]"
+
+abbreviation flatten_values :: "ceclosure heap \<Rightarrow> nat heap" where
+  "flatten_values h \<equiv> hsplay flatten_closure h"
+
+primrec flatten_env :: "(ptr \<times> ptr) \<Rightarrow> ptr list" where
+  "flatten_env (a, b) = [b, a]"
+
+abbreviation flatten_environment :: "(ptr \<times> ptr) heap \<Rightarrow> ptr heap" where
+  "flatten_environment h \<equiv> hsplay flatten_env h"
+
+primrec flatten_frame :: "(ptr \<times> nat) \<Rightarrow> nat list" where
+  "flatten_frame (a, b) = [b, 2 * a]"
+
+abbreviation flatten_stack :: "(ptr \<times> nat) list \<Rightarrow> nat list" where
+  "flatten_stack sfs \<equiv> concat (map flatten_frame sfs)"
+
 primrec flatten :: "chained_state \<Rightarrow> flat_state" where
-  "flatten (CES h env vs sfs cd) = undefined"
+  "flatten (CES h env vs sfs cd) = 
+      FS (flatten_values h) (flatten_environment env) vs (flatten_stack sfs) cd"
+
+lemma [simp]: "get_closure (flatten_values h) v = hlookup h v"
+  by simp
+
+lemma [simp]: "length (flatten_env e) = 2"
+  by (induction e) simp_all
+
+lemma [simp]: "fst e = flatten_env e ! 1"
+  by (induction e) simp_all
+
+lemma [simp]: "snd e = flatten_env e ! 0"
+  by (induction e) simp_all
+
+lemma [simp]: "flat_lookup (flatten_environment env) (2 * p) x = chain_lookup env p x"
+  by (induction env p x rule: chain_lookup.induct) simp_all
+
+lemma flatten_halloc [simp]: "halloc h c = (h', v) \<Longrightarrow> 
+    halloc_list (flatten_values h) (flatten_closure c) = (flatten_values h', v)"
+  by simp
 
 theorem correctf: "flatten \<Sigma>\<^sub>c\<^sub>e \<leadsto>\<^sub>f \<Sigma>\<^sub>f' \<Longrightarrow> \<exists>\<Sigma>\<^sub>c\<^sub>e'. \<Sigma>\<^sub>c\<^sub>e \<leadsto>\<^sub>c\<^sub>e \<Sigma>\<^sub>c\<^sub>e' \<and> flatten \<Sigma>\<^sub>c\<^sub>e' = \<Sigma>\<^sub>f'" 
   by simp
 
 theorem completef [simp]: "\<Sigma>\<^sub>c\<^sub>e \<leadsto>\<^sub>c\<^sub>e \<Sigma>\<^sub>c\<^sub>e' \<Longrightarrow> flatten \<Sigma>\<^sub>c\<^sub>e \<leadsto>\<^sub>f flatten \<Sigma>\<^sub>c\<^sub>e'" 
-  by simp
+proof (induction \<Sigma>\<^sub>c\<^sub>e \<Sigma>\<^sub>c\<^sub>e' rule: evalce.induct)
+  case (evce_pushcon cd pc k h h' v env vs p sfs)
+  moreover hence "halloc_list (flatten_values h) [0, k, 0] = (flatten_values h', v)" 
+    using flatten_halloc by fastforce
+  ultimately show ?case by simp
+next
+  case (evce_pushlam cd pc pc' h p h' v env vs sfs)
+  moreover hence "halloc_list (flatten_values h) [1, 2 * p, pc'] = (flatten_values h', v)" 
+    using flatten_halloc by fastforce
+  ultimately show ?case by simp
+next
+  case (evce_apply cd pc h v2 p' pc' env v1 env' p'' vs p sfs)
+  then show ?case by simp
+next
+  case (evce_jump cd pc h v2 p' pc' env v1 env' p'' vs p sfs)
+  then show ?case by simp
+qed simp_all
 
 lemma completef_iter [simp]: "iter (\<leadsto>\<^sub>c\<^sub>e) \<Sigma>\<^sub>c\<^sub>e \<Sigma>\<^sub>c\<^sub>e' \<Longrightarrow> iter (\<leadsto>\<^sub>f) (flatten \<Sigma>\<^sub>c\<^sub>e) (flatten \<Sigma>\<^sub>c\<^sub>e')"
 proof (induction \<Sigma>\<^sub>c\<^sub>e \<Sigma>\<^sub>c\<^sub>e' rule: iter.induct)
