12UnstructuredMemory/UnstructuredMemory.thy
@@ -1,69 +1,75 @@
 theory UnstructuredMemory
-  imports "../08HeapMemory/HeapMemory"
+  imports "../10ChainedEnvironment/ChainedEnvironment"
 begin
 
 datatype unstr_state = 
-  US (heap: "nat \<Rightarrow> nat") (heap_pointer: nat) ("values": "nat \<Rightarrow> nat") (value_pointer: nat) 
-     (callstack: "nat \<Rightarrow> nat") (callstack_pointer: nat) (code_pointer: nat) (code: "byte_code list")
-
-primrec ulookup_list :: "(nat \<Rightarrow> nat) \<Rightarrow> nat \<Rightarrow> nat \<Rightarrow> nat list" where
-  "ulookup_list h x 0 = []"
-| "ulookup_list h x (Suc n) = h x # ulookup_list h (Suc x) n"
-
-primrec ualloc_list :: "(nat \<Rightarrow> nat) \<Rightarrow> nat \<Rightarrow> nat list \<Rightarrow> (nat \<Rightarrow> nat)" where
-  "ualloc_list h hp [] = h"
-| "ualloc_list h hp (x # xs) = ualloc_list (h(hp := x)) (Suc hp) xs"
-
-fun uget_closure :: "(nat \<Rightarrow> nat) \<Rightarrow> nat \<Rightarrow> hclosure" where
-  "uget_closure h p = (case h p of
-      0 \<Rightarrow> HConst (h (Suc p))
-    | Suc x \<Rightarrow> HLam (ulookup_list h (Suc (Suc p)) x) (h (Suc p)))"
+  US "nat \<Rightarrow> nat" nat nat nat "nat \<Rightarrow> nat" nat "nat \<Rightarrow> nat" nat "nat \<Rightarrow> nat" nat nat 
+     (code: "byte_code list")
 
 inductive evalu :: "unstr_state \<Rightarrow> unstr_state \<Rightarrow> bool" (infix "\<leadsto>\<^sub>u" 50) where
-  evu_lookup [simp]: "cd ! pc = BLookup x \<Longrightarrow>
-    US h hp vs vp sh sp (Suc pc) cd \<leadsto>\<^sub>u US h hp (vs(vp := sh (sp - Suc x))) (Suc vp) sh sp pc cd"
-| evu_pushcon [simp]: "cd ! pc = BPushCon k \<Longrightarrow> 
-    US h hp vs vp sh sp (Suc pc) cd \<leadsto>\<^sub>u 
-      US (ualloc_list h hp [0, k]) (hp + 2) (vs(vp := hp)) (Suc vp) sh sp pc cd"
-| evf_pushlam [simp]: "cd ! pc = BPushLam pc' d \<Longrightarrow> 
-   US h hp vs vp sh sp (Suc pc) cd \<leadsto>\<^sub>u 
-      US (ualloc_list h hp (Suc d # pc' # env)) (hp + d + 2) (vs(vp := hp)) (Suc vp) sh sp pc cd"
-| evf_apply [simp]: "cd ! pc = BApply \<Longrightarrow> uget_closure h (vs (vp - 2)) = HLam env' pc' \<Longrightarrow>
-    US h hp vs vp sh sp (Suc pc) cd \<leadsto>\<^sub>u US h hp vs (vp - 2) 
-      (ualloc_list (sh(sp := pc, sp + length env' + 1 := vs (vp - 1))) (Suc sp) env')
-        (sp + length env' + 2) pc' cd"
-| evf_return [simp]: "cd ! pc = BReturn d \<Longrightarrow> 
-    US h hp vs vp sh sp (Suc pc) cd \<leadsto>\<^sub>u US h hp vs vp sh (sp - d) (sh(sp - d)) cd"
-| evf_jump [simp]: "cd ! pc = BJump d \<Longrightarrow> uget_closure h (vs (vp - 2)) = HLam env' pc' \<Longrightarrow>
-    US h hp vs vp sh sp (Suc pc) cd \<leadsto>\<^sub>u US h hp vs (vp - 2) 
-      (ualloc_list (sh(sp - d + length env' + 1 := vs (vp - 1))) (sp - d + 1) env')
-        (sp - d + length env' + 2) pc' cd"
+  evu_lookup_init [simp]: "cd ! pc = BLookup x \<Longrightarrow> 
+    US h hp 0 0 e ep vs vp sh sp (Suc pc) cd \<leadsto>\<^sub>u 
+      US h hp (Suc x) (sh (sp - 1)) e ep vs vp sh sp (Suc pc) cd"
+| evu_lookup_suc [simp]: "cd ! pc = BLookup y \<Longrightarrow> 
+    US h hp (Suc (Suc x)) (Suc (Suc p)) e ep vs vp sh sp (Suc pc) cd \<leadsto>\<^sub>u 
+      US h hp x (h (Suc p)) e ep vs vp sh sp (Suc pc) cd"
+| evu_lookup_zero [simp]: "cd ! pc = BLookup x \<Longrightarrow> 
+    US h hp (Suc 0) (Suc (Suc p)) e ep vs vp sh sp (Suc pc) cd \<leadsto>\<^sub>u 
+      US h hp 0 0 e ep (vs(vp := h p)) (Suc vp) sh sp pc cd"
+| evu_pushcon [simp]: "cd ! pc = BPushCon k \<Longrightarrow> US h hp x p e ep vs vp sh sp (Suc pc) cd \<leadsto>\<^sub>u 
+    US (h(hp := 0, Suc hp := k, Suc (Suc hp) := 0)) (3 + hp) x p e ep 
+      (vs(vp := hp)) (Suc vp) sh sp pc cd"
+| evu_pushlam [simp]: "cd ! pc = BPushLam pc' \<Longrightarrow> US h hp x p e ep vs vp sh sp (Suc pc) cd \<leadsto>\<^sub>u 
+   US (h(hp := 1, Suc hp := (sh (sp - 1)), Suc (Suc hp) := pc')) (3 + hp) x p e ep 
+      (vs(vp := hp)) (Suc vp) sh sp pc cd"
+| evu_apply [simp]: "cd ! pc = BApply \<Longrightarrow> h (vs (vp - 2)) = 1 \<Longrightarrow> 
+    US h hp x p e ep vs vp sh sp (Suc pc) cd \<leadsto>\<^sub>u 
+      US h hp x p (e(ep := vs (vp - 1), Suc ep := h (Suc (vs (vp - 2))))) (2 + ep) vs (vp - 2) 
+        (sh(sp := Suc (Suc ep), Suc sp := h (Suc (Suc (vs (vp - 2)))))) (2 + sp) pc cd"
+| evu_return [simp]: "cd ! pc = BReturn \<Longrightarrow> 
+    US h hp x p e ep vs vp sh sp (Suc pc) cd \<leadsto>\<^sub>u US h hp x p e ep vs vp sh (sp - 1) (sh(sp - 1)) cd"
+| evu_jump [simp]: "cd ! pc = BJump \<Longrightarrow> h (vs (vp - 2)) = 1 \<Longrightarrow> 
+    US h hp x p e ep vs vp sh sp (Suc pc) cd \<leadsto>\<^sub>u 
+      US h hp x p (e(ep := vs (vp - 1), Suc ep := h (Suc (vs (vp - 2))))) (2 + ep) vs (vp - 2) 
+        (sh(sp - 2 := Suc (Suc ep), sp - 1 := h (Suc (Suc (vs (vp - 2)))))) sp pc cd"
 
 theorem determinismu: "\<Sigma> \<leadsto>\<^sub>u \<Sigma>' \<Longrightarrow> \<Sigma> \<leadsto>\<^sub>u \<Sigma>'' \<Longrightarrow> \<Sigma>' = \<Sigma>''"
 proof (induction \<Sigma> \<Sigma>' rule: evalu.induct)
-  case (evu_lookup cd pc x h hp vs vp sh sp)
-  from evu_lookup(2, 1) show ?case 
-    by (induction "US h hp vs vp sh sp (Suc pc) cd" \<Sigma>'' rule: evalu.induct) simp_all
+  case (evu_lookup_init cd pc x h hp e ep vs vp sh sp)
+  from evu_lookup_init(2, 1) show ?case 
+    by (induction "US h hp 0 0 e ep vs vp sh sp (Suc pc) cd" \<Sigma>'' rule: evalu.induct) simp_all
 next
-  case (evu_pushcon cd pc k h hp vs vp sh sp)
+  case (evu_lookup_suc cd pc y h hp x p e ep vs vp sh sp)
+  from evu_lookup_suc(2, 1) show ?case 
+    by (induction "US h hp (Suc (Suc x)) (Suc (Suc p)) e ep vs vp sh sp (Suc pc) cd" \<Sigma>'' 
+        rule: evalu.induct) 
+       simp_all
+next
+  case (evu_lookup_zero cd pc x h hp p e ep vs vp sh sp)
+  from evu_lookup_zero(2, 1) show ?case 
+    by (induction "US h hp (Suc 0) (Suc (Suc p)) e ep vs vp sh sp (Suc pc) cd" \<Sigma>'' 
+        rule: evalu.induct) 
+       simp_all
+next
+  case (evu_pushcon cd pc k h hp x p e ep vs vp sh sp)
   from evu_pushcon(2, 1) show ?case 
-    by (induction "US h hp vs vp sh sp (Suc pc) cd" \<Sigma>'' rule: evalu.induct) simp_all
+    by (induction "US h hp x p e ep vs vp sh sp (Suc pc) cd" \<Sigma>'' rule: evalu.induct) simp_all
 next
-  case (evf_pushlam cd pc pc' d h hp vs vp sh sp env)
-  from evf_pushlam(2, 1) show ?case 
-    by (induction "US h hp vs vp sh sp (Suc pc) cd" \<Sigma>'' rule: evalu.induct) simp_all
+  case (evu_pushlam cd pc pc' h hp x p e ep vs vp sh sp)
+  from evu_pushlam(2, 1) show ?case 
+    by (induction "US h hp x p e ep vs vp sh sp (Suc pc) cd" \<Sigma>'' rule: evalu.induct) simp_all
 next
-  case (evf_apply cd pc h vs vp env' pc' hp sh sp)
-  from evf_apply(3, 1, 2) show ?case 
-    by (induction "US h hp vs vp sh sp (Suc pc) cd" \<Sigma>'' rule: evalu.induct) simp_all
+  case (evu_apply cd pc h vs vp hp x p e ep sh sp)
+  from evu_apply(3, 1, 2) show ?case    
+    by (induction "US h hp x p e ep vs vp sh sp (Suc pc) cd" \<Sigma>'' rule: evalu.induct) simp_all
 next
-  case (evf_return cd pc d h hp vs vp sh sp)
-  from evf_return(2, 1) show ?case 
-    by (induction "US h hp vs vp sh sp (Suc pc) cd" \<Sigma>'' rule: evalu.induct) simp_all
+  case (evu_return cd pc h hp x p e ep vs vp sh sp)
+  from evu_return(2, 1) show ?case 
+    by (induction "US h hp x p e ep vs vp sh sp (Suc pc) cd" \<Sigma>'' rule: evalu.induct) simp_all
 next
-  case (evf_jump cd pc d h vs vp env' pc' hp sh sp)
-  from evf_jump(3, 1, 2) show ?case 
-    by (induction "US h hp vs vp sh sp (Suc pc) cd" \<Sigma>'' rule: evalu.induct) simp_all
+  case (evu_jump cd pc h vs vp hp x p e ep sh sp)
+  from evu_jump(3, 1, 2) show ?case    
+    by (induction "US h hp x p e ep vs vp sh sp (Suc pc) cd" \<Sigma>'' rule: evalu.induct) simp_all
 qed
 
 lemma [simp]: "\<Sigma> \<leadsto>\<^sub>u \<Sigma>' \<Longrightarrow> code \<Sigma> = code \<Sigma>'"
